% vim: spl=en
\begin{problem}{Gordon identity}{p2}
   Show that 
   \begin{equation*}
      \bar{u}(k) \gamma^\mu u(p) = \bar{u}(k) \left[\frac{k^\mu + p^\mu}{2m} + \frac{i \sigma^{\mu \nu} q_\nu}{2m}\right]u(p),
   \end{equation*}
   where \(q = k - p.\)
\end{problem}
\begin{proof}
   Recall that \(\anticommutator{\gamma^\mu}{\gamma^\nu} = 2g^{\mu \nu}\unity,\) then we may write
   \begin{align*}
      i\sigma^{\mu \nu} &= -\frac{1}2 \commutator{\gamma^\mu}{\gamma^\nu} = - \gamma^\mu \gamma^\nu + \frac12\anticommutator{\gamma^\mu}{\gamma^\nu} = g^{\mu \nu}\unity - \gamma^\mu \gamma^\nu\\
                        &= \frac12 \commutator{\gamma^\nu}{\gamma^\mu} = \gamma^\nu \gamma^\mu - \frac12 \anticommutator{\gamma^\nu}{\gamma^\mu} = \gamma^\nu \gamma^\mu - g^{\mu\nu} \unity.
   \end{align*}
   % from which we conclude
   % \begin{equation*}
   %    \gamma^\mu \gamma^\nu = g^{\nu \mu} \unity + i \sigma^{\nu \mu} = g^{\mu\nu} \unity - i \sigma^{\mu\nu}.
   % \end{equation*}
   Let \(q = k - p,\) then
   \begin{align*}
      i \sigma^{\mu\nu} q_\nu &=  (\gamma^\nu \gamma^\mu - g^{\mu \nu} \unity)k_\nu -  (g^{\mu \nu}\unity - \gamma^\mu \gamma^\nu)p_\nu\\
                              &= (\gamma^\nu k_\nu \gamma^\mu - k^\mu \unity) - (p^\mu \unity - \gamma^\mu \gamma^\nu p_\nu)\\
                              &= \slashed{k} \gamma^\mu + \gamma^\mu \slashed{p} - (k^\mu + p^\mu)\unity
   \end{align*}
   hence
   \begin{align*}
      \bar{u}(k) i \sigma^{\mu\nu} q_\nu u(p) &= (\bar{u}(k) \slashed{k})\gamma^\mu u(p) + \bar{u}(k) \gamma^\mu (\slashed{p} u(p)) - \bar{u}(k) (k^\mu + p^\mu) u(p)\\
                                              &= 2m \bar{u}(k) \gamma^\mu u(p) - \bar{u}(k) (k^\mu + p^\mu) u(p)
   \end{align*}
   as \(\slashed{p}u(p) = m u(p)\) and \(\bar{u}(k) \slashed{k} = m \bar{u}(k)\). Assuming \(m \neq 0,\)
   \begin{align*}
      \bar{u}(k) \gamma^\mu u(p) &= \frac{1}{2m}\left[\bar{u}(k) (k^\mu + p^\mu) u(p) + \bar{u}(k) i \sigma^{\mu \nu} q_\nu u(p)\right]\\
                                 &= \bar{u}(k) \left[\frac{k^\mu + p^\mu}{2m} + \frac{i \sigma^{\mu \nu} q_\nu}{2m}\right]u(p)
   \end{align*}
   as desired.
\end{proof}
